examples/MapVReify.v
@@ -341,12 +341,13 @@ Ltac mapVR_Meths n m := mapVReify SignT (fun k (v: SignT k) => v)
 
 Ltac mkStruct :=
   repeat match goal with
-           | H: context[mkStruct ?p ?q] |- _ => rewrite (mkStruct_eq p q) in H;
+           | H: context[@mkStruct ?a ?b ?c] |- _ => rewrite (@mkStruct_eq a b c) in H;
                simpl in H; unfold StringBound.ith_Bounded in H; simpl in H
-           | |- context[mkStruct ?p ?q] => rewrite (mkStruct_eq p q);
+           | |- context[@mkStruct ?a ?b ?c] => rewrite (@mkStruct_eq a b c);
                simpl; unfold StringBound.ith_Bounded; simpl
          end.
 
+(*
 Ltac existRegs n :=
   match goal with
     | |- ?inv ?s =>
@@ -370,7 +371,7 @@ Ltac existRegs n :=
 Ltac simplifyInvs :=
   repeat autounfold with MethDefs in *;
   intros; try (exfalso; assumption);
-  repeat (rewrite ?mapVec_replicate_commute, ?evalVec_replicate in *; simpl in *);
+  repeat (rewrite ?mapVec_replicate_commute, ?evalVec_replicate in *; simpl in * );
   dest; auto; try discriminate;
   repeat match goal with
            | H: nil = (?a ++ ?b :: ?c)%list |- _ => apply app_cons_not_nil in H
@@ -384,8 +385,9 @@ Ltac simplifyInvs :=
 
 Ltac prelimSimplRegs n :=
   existRegs n; simplifyInvs.
+*)
 
-Ltac allRules :=
+Ltac simplMapUpds tac :=
   esplit;
   unfold withIndex;
   match goal with
@@ -404,9 +406,10 @@ Ltac allRules :=
       destruct (eq_nat_dec x x) as [isEq | isEq];
         [ | clear - isEq; intuition auto]
     | _ => idtac
-  end.
+  end; (reflexivity || eassumption || tac).
 
 
+  
 (*
 Ltac initRed :=
   kinv_action_dest;
